<?xml version="1.0"?>
<rdf:RDF xmlns="http://www.semanticweb.org/danielperez-milasanchez/ontologies/2023/3/untitled-ontology-5#"
     xml:base="http://www.semanticweb.org/danielperez-milasanchez/ontologies/2023/3/untitled-ontology-5"
     xmlns:owl="http://www.w3.org/2002/07/owl#"
     xmlns:rdf="http://www.w3.org/1999/02/22-rdf-syntax-ns#"
     xmlns:xml="http://www.w3.org/XML/1998/namespace"
     xmlns:xsd="http://www.w3.org/2001/XMLSchema#"
     xmlns:rdfs="http://www.w3.org/2000/01/rdf-schema#"
     xmlns:swrl="http://www.w3.org/2003/11/swrl#"
     xmlns:swrlb="http://www.w3.org/2003/11/swrlb#"
     xmlns:untitled-ontology-5="http://www.semanticweb.org/danielperez-milasanchez/ontologies/2023/3/untitled-ontology-5#">
    <owl:Ontology rdf:about="http://www.semanticweb.org/danielperez-milasanchez/ontologies/2023/3/untitled-ontology-5">
        <rdfs:comment>1. Title: Spanish Wine Checker Ontology</rdfs:comment>
        <rdfs:comment>2. Author: Daniel Pérez-Milá Sánchez</rdfs:comment>
        <rdfs:comment>3. Description: This ontology is about Spanish wines and their characteristics.</rdfs:comment>
        <owl:versionInfo rdf:datatype="http://www.w3.org/2001/XMLSchema#decimal">1.0</owl:versionInfo>
    </owl:Ontology>
    


    <!-- 
    ///////////////////////////////////////////////////////////////////////////////////////
    //
    // Object Properties
    //
    ///////////////////////////////////////////////////////////////////////////////////////
     -->


    


    <!-- http://www.semanticweb.org/danielperez-milasanchez/ontologies/2023/3/untitled-ontology-5#isComposedOf -->


    <owl:ObjectProperty rdf:about="http://www.semanticweb.org/danielperez-milasanchez/ontologies/2023/3/untitled-ontology-5#isComposedOf">
        <rdfs:domain rdf:resource="http://www.semanticweb.org/danielperez-milasanchez/ontologies/2023/3/untitled-ontology-5#Wine"/>
        <rdfs:range rdf:resource="http://www.semanticweb.org/danielperez-milasanchez/ontologies/2023/3/untitled-ontology-5#Grape"/>
        <rdfs:comment>A type of wine is made from one or more grape varieties.</rdfs:comment>
    </owl:ObjectProperty>
    


    <!-- http://www.semanticweb.org/danielperez-milasanchez/ontologies/2023/3/untitled-ontology-5#isGrownIn -->


    <owl:ObjectProperty rdf:about="http://www.semanticweb.org/danielperez-milasanchez/ontologies/2023/3/untitled-ontology-5#isGrownIn">
        <rdfs:domain rdf:resource="http://www.semanticweb.org/danielperez-milasanchez/ontologies/2023/3/untitled-ontology-5#Grape"/>
        <rdfs:range rdf:resource="http://www.semanticweb.org/danielperez-milasanchez/ontologies/2023/3/untitled-ontology-5#Spanish_region"/>
        <rdfs:comment>A grape variety is grown in one or more Spanish regions.</rdfs:comment>
    </owl:ObjectProperty>
    


    <!-- http://www.semanticweb.org/danielperez-milasanchez/ontologies/2023/3/untitled-ontology-5#isMadeIn -->


    <owl:ObjectProperty rdf:about="http://www.semanticweb.org/danielperez-milasanchez/ontologies/2023/3/untitled-ontology-5#isMadeIn">
        <rdfs:domain rdf:resource="http://www.semanticweb.org/danielperez-milasanchez/ontologies/2023/3/untitled-ontology-5#Wine"/>
        <rdfs:range rdf:resource="http://www.semanticweb.org/danielperez-milasanchez/ontologies/2023/3/untitled-ontology-5#Spanish_region"/>
        <rdfs:comment>A type of wine is produced in one or more Spanish regions.</rdfs:comment>
    </owl:ObjectProperty>
    


    <!-- 
    ///////////////////////////////////////////////////////////////////////////////////////
    //
    // Data properties
    //
    ///////////////////////////////////////////////////////////////////////////////////////
     -->


    


    <!-- http://www.semanticweb.org/danielperez-milasanchez/ontologies/2023/3/untitled-ontology-5#hasAcidityLevel -->


    <owl:DatatypeProperty rdf:about="http://www.semanticweb.org/danielperez-milasanchez/ontologies/2023/3/untitled-ontology-5#hasAcidityLevel">
        <rdfs:domain rdf:resource="http://www.semanticweb.org/danielperez-milasanchez/ontologies/2023/3/untitled-ontology-5#Wine"/>
        <rdfs:range rdf:resource="http://www.w3.org/2001/XMLSchema#int"/>
        <rdfs:comment>A type of wine has a specific level of acidity when tasted within a range of 1 to 5.</rdfs:comment>
    </owl:DatatypeProperty>
    


    <!-- http://www.semanticweb.org/danielperez-milasanchez/ontologies/2023/3/untitled-ontology-5#hasAlcoholDegree -->


    <owl:DatatypeProperty rdf:about="http://www.semanticweb.org/danielperez-milasanchez/ontologies/2023/3/untitled-ontology-5#hasAlcoholDegree">
        <rdfs:domain rdf:resource="http://www.semanticweb.org/danielperez-milasanchez/ontologies/2023/3/untitled-ontology-5#Wine"/>
        <rdfs:range rdf:resource="http://www.w3.org/2001/XMLSchema#float"/>
        <rdfs:comment>A type of wine has a specific alcohol degree within a range of 0% to 100%.</rdfs:comment>
    </owl:DatatypeProperty>
    


    <!-- http://www.semanticweb.org/danielperez-milasanchez/ontologies/2023/3/untitled-ontology-5#hasBodyLevel -->


    <owl:DatatypeProperty rdf:about="http://www.semanticweb.org/danielperez-milasanchez/ontologies/2023/3/untitled-ontology-5#hasBodyLevel">
        <rdfs:domain rdf:resource="http://www.semanticweb.org/danielperez-milasanchez/ontologies/2023/3/untitled-ontology-5#Wine"/>
        <rdfs:range rdf:resource="http://www.w3.org/2001/XMLSchema#int"/>
        <rdfs:comment>A type of wine has a specific level of body when tasted within a range of 1 to 5.</rdfs:comment>
    </owl:DatatypeProperty>
    


    <!-- 
    ///////////////////////////////////////////////////////////////////////////////////////
    //
    // Classes
    //
    ///////////////////////////////////////////////////////////////////////////////////////
     -->


    


    <!-- http://www.semanticweb.org/danielperez-milasanchez/ontologies/2023/3/untitled-ontology-5#Albarino_white_grape -->


    <owl:Class rdf:about="http://www.semanticweb.org/danielperez-milasanchez/ontologies/2023/3/untitled-ontology-5#Albarino_white_grape">
        <rdfs:subClassOf rdf:resource="http://www.semanticweb.org/danielperez-milasanchez/ontologies/2023/3/untitled-ontology-5#White_grape"/>
        <rdfs:comment>A type of white grape used to make a particular white or sparkling wine.</rdfs:comment>
    </owl:Class>
    


    <!-- http://www.semanticweb.org/danielperez-milasanchez/ontologies/2023/3/untitled-ontology-5#Albarino_wine -->


    <owl:Class rdf:about="http://www.semanticweb.org/danielperez-milasanchez/ontologies/2023/3/untitled-ontology-5#Albarino_wine">
        <rdfs:subClassOf rdf:resource="http://www.semanticweb.org/danielperez-milasanchez/ontologies/2023/3/untitled-ontology-5#White_wine"/>
        <rdfs:comment>Albariño wine (“alba-reen-yo”) is a delightfully refreshing coastal white that grows on the Iberian Peninsula. It’s loved for its rich stone fruit flavors, a hint of salinity, and zippy acidity.</rdfs:comment>
    </owl:Class>
    


    <!-- http://www.semanticweb.org/danielperez-milasanchez/ontologies/2023/3/untitled-ontology-5#Andalusia -->


    <owl:Class rdf:about="http://www.semanticweb.org/danielperez-milasanchez/ontologies/2023/3/untitled-ontology-5#Andalusia">
        <rdfs:subClassOf rdf:resource="http://www.semanticweb.org/danielperez-milasanchez/ontologies/2023/3/untitled-ontology-5#Spanish_region"/>
    </owl:Class>
    


    <!-- http://www.semanticweb.org/danielperez-milasanchez/ontologies/2023/3/untitled-ontology-5#Aragon -->


    <owl:Class rdf:about="http://www.semanticweb.org/danielperez-milasanchez/ontologies/2023/3/untitled-ontology-5#Aragon">
        <rdfs:subClassOf rdf:resource="http://www.semanticweb.org/danielperez-milasanchez/ontologies/2023/3/untitled-ontology-5#Spanish_region"/>
        <rdfs:comment>It is an Autonomous Community of Spain where grapes are grown for wine production.</rdfs:comment>
    </owl:Class>
    


    <!-- http://www.semanticweb.org/danielperez-milasanchez/ontologies/2023/3/untitled-ontology-5#Balearic_Islands -->


    <owl:Class rdf:about="http://www.semanticweb.org/danielperez-milasanchez/ontologies/2023/3/untitled-ontology-5#Balearic_Islands">
        <rdfs:subClassOf rdf:resource="http://www.semanticweb.org/danielperez-milasanchez/ontologies/2023/3/untitled-ontology-5#Spanish_region"/>
        <rdfs:comment>It is an Autonomous Community of Spain where grapes are grown for wine production.</rdfs:comment>
    </owl:Class>
    


    <!-- http://www.semanticweb.org/danielperez-milasanchez/ontologies/2023/3/untitled-ontology-5#Basque_Country -->


    <owl:Class rdf:about="http://www.semanticweb.org/danielperez-milasanchez/ontologies/2023/3/untitled-ontology-5#Basque_Country">
        <rdfs:subClassOf rdf:resource="http://www.semanticweb.org/danielperez-milasanchez/ontologies/2023/3/untitled-ontology-5#Spanish_region"/>
        <rdfs:comment>It is an Autonomous Community of Spain where grapes are grown for wine production.</rdfs:comment>
    </owl:Class>
    


    <!-- http://www.semanticweb.org/danielperez-milasanchez/ontologies/2023/3/untitled-ontology-5#Cabernet_Franc_red_grape -->


    <owl:Class rdf:about="http://www.semanticweb.org/danielperez-milasanchez/ontologies/2023/3/untitled-ontology-5#Cabernet_Franc_red_grape">
        <rdfs:subClassOf rdf:resource="http://www.semanticweb.org/danielperez-milasanchez/ontologies/2023/3/untitled-ontology-5#Red_grape"/>
        <rdfs:comment>A type of red grape used to make a particular red wine.</rdfs:comment>
    </owl:Class>
    


    <!-- http://www.semanticweb.org/danielperez-milasanchez/ontologies/2023/3/untitled-ontology-5#Cabernet_Sauvignon_red_grape -->


    <owl:Class rdf:about="http://www.semanticweb.org/danielperez-milasanchez/ontologies/2023/3/untitled-ontology-5#Cabernet_Sauvignon_red_grape">
        <rdfs:subClassOf rdf:resource="http://www.semanticweb.org/danielperez-milasanchez/ontologies/2023/3/untitled-ontology-5#Red_grape"/>
        <rdfs:comment>A type of red grape used to make a particular red wine.</rdfs:comment>
    </owl:Class>
    


    <!-- http://www.semanticweb.org/danielperez-milasanchez/ontologies/2023/3/untitled-ontology-5#Cabernet_Sauvignon_wine -->


    <owl:Class rdf:about="http://www.semanticweb.org/danielperez-milasanchez/ontologies/2023/3/untitled-ontology-5#Cabernet_Sauvignon_wine">
        <owl:equivalentClass>
            <owl:Restriction>
                <owl:onProperty rdf:resource="http://www.semanticweb.org/danielperez-milasanchez/ontologies/2023/3/untitled-ontology-5#hasAcidityLevel"/>
                <owl:someValuesFrom>
                    <rdfs:Datatype>
                        <owl:oneOf>
                            <rdf:Description>
                                <rdf:type rdf:resource="http://www.w3.org/1999/02/22-rdf-syntax-ns#List"/>
                                <rdf:first rdf:datatype="http://www.w3.org/2001/XMLSchema#integer">5</rdf:first>
                                <rdf:rest rdf:resource="http://www.w3.org/1999/02/22-rdf-syntax-ns#nil"/>
                            </rdf:Description>
                        </owl:oneOf>
                    </rdfs:Datatype>
                </owl:someValuesFrom>
            </owl:Restriction>
        </owl:equivalentClass>
        <rdfs:subClassOf rdf:resource="http://www.semanticweb.org/danielperez-milasanchez/ontologies/2023/3/untitled-ontology-5#Montsant_Red_wine"/>
        <rdfs:subClassOf rdf:resource="http://www.semanticweb.org/danielperez-milasanchez/ontologies/2023/3/untitled-ontology-5#Priorat_Red_wine"/>
        <rdfs:subClassOf rdf:resource="http://www.semanticweb.org/danielperez-milasanchez/ontologies/2023/3/untitled-ontology-5#Red_wine"/>
        <rdfs:subClassOf rdf:resource="http://www.semanticweb.org/danielperez-milasanchez/ontologies/2023/3/untitled-ontology-5#Ribera_del_Duero_Red_wine"/>
        <rdfs:comment>The world’s most popular red wine grape is a natural cross between Cabernet Franc and Sauvignon Blanc from Bordeaux, France. Cabernet Sauvignon is loved for its high concentration and age worthiness.</rdfs:comment>
    </owl:Class>
    


    <!-- http://www.semanticweb.org/danielperez-milasanchez/ontologies/2023/3/untitled-ontology-5#Canary_Islands -->


    <owl:Class rdf:about="http://www.semanticweb.org/danielperez-milasanchez/ontologies/2023/3/untitled-ontology-5#Canary_Islands">
        <rdfs:subClassOf rdf:resource="http://www.semanticweb.org/danielperez-milasanchez/ontologies/2023/3/untitled-ontology-5#Spanish_region"/>
        <rdfs:comment>It is an Autonomous Community of Spain where grapes are grown for wine production.</rdfs:comment>
    </owl:Class>
    


    <!-- http://www.semanticweb.org/danielperez-milasanchez/ontologies/2023/3/untitled-ontology-5#Carignan_red_grape -->


    <owl:Class rdf:about="http://www.semanticweb.org/danielperez-milasanchez/ontologies/2023/3/untitled-ontology-5#Carignan_red_grape">
        <rdfs:subClassOf rdf:resource="http://www.semanticweb.org/danielperez-milasanchez/ontologies/2023/3/untitled-ontology-5#Red_grape"/>
        <rdfs:comment>A type of red grape used to make a particular red wine.</rdfs:comment>
    </owl:Class>
    


    <!-- http://www.semanticweb.org/danielperez-milasanchez/ontologies/2023/3/untitled-ontology-5#Castile-La_Mancha -->


    <owl:Class rdf:about="http://www.semanticweb.org/danielperez-milasanchez/ontologies/2023/3/untitled-ontology-5#Castile-La_Mancha">
        <rdfs:subClassOf rdf:resource="http://www.semanticweb.org/danielperez-milasanchez/ontologies/2023/3/untitled-ontology-5#Spanish_region"/>
        <rdfs:comment>It is an Autonomous Community of Spain where grapes are grown for wine production.</rdfs:comment>
    </owl:Class>
    


    <!-- http://www.semanticweb.org/danielperez-milasanchez/ontologies/2023/3/untitled-ontology-5#Castile_and_Leon -->


    <owl:Class rdf:about="http://www.semanticweb.org/danielperez-milasanchez/ontologies/2023/3/untitled-ontology-5#Castile_and_Leon">
        <rdfs:subClassOf rdf:resource="http://www.semanticweb.org/danielperez-milasanchez/ontologies/2023/3/untitled-ontology-5#Spanish_region"/>
        <rdfs:comment>It is an Autonomous Community of Spain where grapes are grown for wine production.</rdfs:comment>
    </owl:Class>
    


    <!-- http://www.semanticweb.org/danielperez-milasanchez/ontologies/2023/3/untitled-ontology-5#Catalonia -->


    <owl:Class rdf:about="http://www.semanticweb.org/danielperez-milasanchez/ontologies/2023/3/untitled-ontology-5#Catalonia">
        <rdfs:subClassOf rdf:resource="http://www.semanticweb.org/danielperez-milasanchez/ontologies/2023/3/untitled-ontology-5#Spanish_region"/>
        <rdfs:comment>It is an Autonomous Community of Spain where grapes are grown for wine production.</rdfs:comment>
    </owl:Class>
    


    <!-- http://www.semanticweb.org/danielperez-milasanchez/ontologies/2023/3/untitled-ontology-5#Cava_wine -->


    <owl:Class rdf:about="http://www.semanticweb.org/danielperez-milasanchez/ontologies/2023/3/untitled-ontology-5#Cava_wine">
        <rdfs:subClassOf rdf:resource="http://www.semanticweb.org/danielperez-milasanchez/ontologies/2023/3/untitled-ontology-5#Sparkling_wine"/>
        <rdfs:comment>Cava is the premier sparkling of Spain. The wine uses a similar quality tier system to Champagne but champions several of Spain’s native grapes including Macabeu (Viura), Xarel-lo, and Parellada.</rdfs:comment>
    </owl:Class>
    


    <!-- http://www.semanticweb.org/danielperez-milasanchez/ontologies/2023/3/untitled-ontology-5#Chardonnay_white_grape -->


    <owl:Class rdf:about="http://www.semanticweb.org/danielperez-milasanchez/ontologies/2023/3/untitled-ontology-5#Chardonnay_white_grape">
        <rdfs:subClassOf rdf:resource="http://www.semanticweb.org/danielperez-milasanchez/ontologies/2023/3/untitled-ontology-5#White_grape"/>
        <rdfs:comment>A type of white grape used to make a particular white or sparkling wine.</rdfs:comment>
    </owl:Class>
    


    <!-- http://www.semanticweb.org/danielperez-milasanchez/ontologies/2023/3/untitled-ontology-5#Chardonnay_wine -->


    <owl:Class rdf:about="http://www.semanticweb.org/danielperez-milasanchez/ontologies/2023/3/untitled-ontology-5#Chardonnay_wine">
        <rdfs:subClassOf rdf:resource="http://www.semanticweb.org/danielperez-milasanchez/ontologies/2023/3/untitled-ontology-5#White_wine"/>
        <rdfs:comment>One of the world’s most popular grapes, Chardonnay is made in a wide range of styles from lean, sparkling Blanc de Blancs to rich, creamy white wines aged in oak.</rdfs:comment>
    </owl:Class>
    


    <!-- http://www.semanticweb.org/danielperez-milasanchez/ontologies/2023/3/untitled-ontology-5#Charelo_white_grape -->


    <owl:Class rdf:about="http://www.semanticweb.org/danielperez-milasanchez/ontologies/2023/3/untitled-ontology-5#Charelo_white_grape">
        <rdfs:subClassOf rdf:resource="http://www.semanticweb.org/danielperez-milasanchez/ontologies/2023/3/untitled-ontology-5#White_grape"/>
        <rdfs:comment>A type of white grape used to make a particular white or sparkling wine.</rdfs:comment>
    </owl:Class>
    


    <!-- http://www.semanticweb.org/danielperez-milasanchez/ontologies/2023/3/untitled-ontology-5#Chenin_blanc_white_grape -->


    <owl:Class rdf:about="http://www.semanticweb.org/danielperez-milasanchez/ontologies/2023/3/untitled-ontology-5#Chenin_blanc_white_grape">
        <rdfs:subClassOf rdf:resource="http://www.semanticweb.org/danielperez-milasanchez/ontologies/2023/3/untitled-ontology-5#White_grape"/>
        <rdfs:comment>A type of white grape used to make a particular white or sparkling wine.</rdfs:comment>
    </owl:Class>
    


    <!-- http://www.semanticweb.org/danielperez-milasanchez/ontologies/2023/3/untitled-ontology-5#Extremadura -->


    <owl:Class rdf:about="http://www.semanticweb.org/danielperez-milasanchez/ontologies/2023/3/untitled-ontology-5#Extremadura">
        <rdfs:subClassOf rdf:resource="http://www.semanticweb.org/danielperez-milasanchez/ontologies/2023/3/untitled-ontology-5#Spanish_region"/>
        <rdfs:comment>It is an Autonomous Community of Spain where grapes are grown for wine production.</rdfs:comment>
    </owl:Class>
    


    <!-- http://www.semanticweb.org/danielperez-milasanchez/ontologies/2023/3/untitled-ontology-5#Galicia -->


    <owl:Class rdf:about="http://www.semanticweb.org/danielperez-milasanchez/ontologies/2023/3/untitled-ontology-5#Galicia">
        <rdfs:subClassOf rdf:resource="http://www.semanticweb.org/danielperez-milasanchez/ontologies/2023/3/untitled-ontology-5#Spanish_region"/>
        <rdfs:comment>It is an Autonomous Community of Spain where grapes are grown for wine production.</rdfs:comment>
    </owl:Class>
    


    <!-- http://www.semanticweb.org/danielperez-milasanchez/ontologies/2023/3/untitled-ontology-5#Graciano_red_grape -->


    <owl:Class rdf:about="http://www.semanticweb.org/danielperez-milasanchez/ontologies/2023/3/untitled-ontology-5#Graciano_red_grape">
        <rdfs:subClassOf rdf:resource="http://www.semanticweb.org/danielperez-milasanchez/ontologies/2023/3/untitled-ontology-5#Red_grape"/>
        <rdfs:comment>A type of red grape used to make a particular red wine.</rdfs:comment>
    </owl:Class>
    


    <!-- http://www.semanticweb.org/danielperez-milasanchez/ontologies/2023/3/untitled-ontology-5#Grape -->


    <owl:Class rdf:about="http://www.semanticweb.org/danielperez-milasanchez/ontologies/2023/3/untitled-ontology-5#Grape">
        <owl:equivalentClass>
            <owl:Restriction>
                <owl:onProperty rdf:resource="http://www.semanticweb.org/danielperez-milasanchez/ontologies/2023/3/untitled-ontology-5#isGrownIn"/>
                <owl:someValuesFrom rdf:resource="http://www.semanticweb.org/danielperez-milasanchez/ontologies/2023/3/untitled-ontology-5#Spanish_region"/>
            </owl:Restriction>
        </owl:equivalentClass>
        <rdfs:comment>A grape is a fruit, botanically a berry, of the deciduous woody vines of the flowering plant genus Vitis. Grapes are a non-climacteric type of fruit, generally occurring in clusters. They are known for the wine production.</rdfs:comment>
    </owl:Class>
    


    <!-- http://www.semanticweb.org/danielperez-milasanchez/ontologies/2023/3/untitled-ontology-5#Grenache_red_grape -->


    <owl:Class rdf:about="http://www.semanticweb.org/danielperez-milasanchez/ontologies/2023/3/untitled-ontology-5#Grenache_red_grape">
        <rdfs:subClassOf rdf:resource="http://www.semanticweb.org/danielperez-milasanchez/ontologies/2023/3/untitled-ontology-5#Red_grape"/>
        <rdfs:comment>A type of red grape used to make a particular red wine.</rdfs:comment>
    </owl:Class>
    


    <!-- http://www.semanticweb.org/danielperez-milasanchez/ontologies/2023/3/untitled-ontology-5#Grenache_white_grape -->


    <owl:Class rdf:about="http://www.semanticweb.org/danielperez-milasanchez/ontologies/2023/3/untitled-ontology-5#Grenache_white_grape">
        <rdfs:subClassOf rdf:resource="http://www.semanticweb.org/danielperez-milasanchez/ontologies/2023/3/untitled-ontology-5#White_grape"/>
        <rdfs:comment>A type of white grape used to make a particular white or sparkling wine.</rdfs:comment>
    </owl:Class>
    


    <!-- http://www.semanticweb.org/danielperez-milasanchez/ontologies/2023/3/untitled-ontology-5#Grenache_wine -->


    <owl:Class rdf:about="http://www.semanticweb.org/danielperez-milasanchez/ontologies/2023/3/untitled-ontology-5#Grenache_wine">
        <rdfs:subClassOf rdf:resource="http://www.semanticweb.org/danielperez-milasanchez/ontologies/2023/3/untitled-ontology-5#Montsant_Red_wine"/>
        <rdfs:subClassOf rdf:resource="http://www.semanticweb.org/danielperez-milasanchez/ontologies/2023/3/untitled-ontology-5#Red_wine"/>
        <rdfs:subClassOf rdf:resource="http://www.semanticweb.org/danielperez-milasanchez/ontologies/2023/3/untitled-ontology-5#Ribera_del_Duero_Red_wine"/>
        <rdfs:subClassOf rdf:resource="http://www.semanticweb.org/danielperez-milasanchez/ontologies/2023/3/untitled-ontology-5#Rioja_Red_wine"/>
        <rdfs:subClassOf rdf:resource="http://www.semanticweb.org/danielperez-milasanchez/ontologies/2023/3/untitled-ontology-5#Toro_Red_wine"/>
        <rdfs:comment>Grenache (aka Garnacha) produces rich, flavorful red wines and deep, ruby-tinted rosé. The French have championed this grape in the Southern Rhône Valley but it’s original home is Spain.</rdfs:comment>
    </owl:Class>
    


    <!-- http://www.semanticweb.org/danielperez-milasanchez/ontologies/2023/3/untitled-ontology-5#La_Rioja -->


    <owl:Class rdf:about="http://www.semanticweb.org/danielperez-milasanchez/ontologies/2023/3/untitled-ontology-5#La_Rioja">
        <rdfs:subClassOf rdf:resource="http://www.semanticweb.org/danielperez-milasanchez/ontologies/2023/3/untitled-ontology-5#Spanish_region"/>
        <rdfs:comment>It is an Autonomous Community of Spain where grapes are grown for wine production.</rdfs:comment>
    </owl:Class>
    


    <!-- http://www.semanticweb.org/danielperez-milasanchez/ontologies/2023/3/untitled-ontology-5#Malbec_red_grape -->


    <owl:Class rdf:about="http://www.semanticweb.org/danielperez-milasanchez/ontologies/2023/3/untitled-ontology-5#Malbec_red_grape">
        <rdfs:subClassOf rdf:resource="http://www.semanticweb.org/danielperez-milasanchez/ontologies/2023/3/untitled-ontology-5#Red_grape"/>
        <rdfs:comment>A type of red grape used to make a particular red wine.</rdfs:comment>
    </owl:Class>
    


    <!-- http://www.semanticweb.org/danielperez-milasanchez/ontologies/2023/3/untitled-ontology-5#Malvasia_white_grape -->


    <owl:Class rdf:about="http://www.semanticweb.org/danielperez-milasanchez/ontologies/2023/3/untitled-ontology-5#Malvasia_white_grape">
        <rdfs:subClassOf rdf:resource="http://www.semanticweb.org/danielperez-milasanchez/ontologies/2023/3/untitled-ontology-5#White_grape"/>
        <rdfs:comment>A type of white grape used to make a particular white or sparkling wine.</rdfs:comment>
    </owl:Class>
    


    <!-- http://www.semanticweb.org/danielperez-milasanchez/ontologies/2023/3/untitled-ontology-5#Mazuelo_red_grape -->


    <owl:Class rdf:about="http://www.semanticweb.org/danielperez-milasanchez/ontologies/2023/3/untitled-ontology-5#Mazuelo_red_grape">
        <rdfs:subClassOf rdf:resource="http://www.semanticweb.org/danielperez-milasanchez/ontologies/2023/3/untitled-ontology-5#Red_grape"/>
        <rdfs:comment>A type of red grape used to make a particular red wine.</rdfs:comment>
    </owl:Class>
    


    <!-- http://www.semanticweb.org/danielperez-milasanchez/ontologies/2023/3/untitled-ontology-5#Mencia_red_grape -->


    <owl:Class rdf:about="http://www.semanticweb.org/danielperez-milasanchez/ontologies/2023/3/untitled-ontology-5#Mencia_red_grape">
        <rdfs:subClassOf rdf:resource="http://www.semanticweb.org/danielperez-milasanchez/ontologies/2023/3/untitled-ontology-5#Red_grape"/>
        <rdfs:comment>A type of red grape used to make a particular red wine.</rdfs:comment>
    </owl:Class>
    


    <!-- http://www.semanticweb.org/danielperez-milasanchez/ontologies/2023/3/untitled-ontology-5#Mencia_wine -->


    <owl:Class rdf:about="http://www.semanticweb.org/danielperez-milasanchez/ontologies/2023/3/untitled-ontology-5#Mencia_wine">
        <rdfs:subClassOf rdf:resource="http://www.semanticweb.org/danielperez-milasanchez/ontologies/2023/3/untitled-ontology-5#Red_wine"/>
        <rdfs:comment>A red variety from the Iberian peninsula (Spain and Portugal) that’s quickly developing a following. It’s loved for its heady aromatics and potential to age.</rdfs:comment>
    </owl:Class>
    


    <!-- http://www.semanticweb.org/danielperez-milasanchez/ontologies/2023/3/untitled-ontology-5#Merlot_red_grape -->


    <owl:Class rdf:about="http://www.semanticweb.org/danielperez-milasanchez/ontologies/2023/3/untitled-ontology-5#Merlot_red_grape">
        <rdfs:subClassOf rdf:resource="http://www.semanticweb.org/danielperez-milasanchez/ontologies/2023/3/untitled-ontology-5#Red_grape"/>
        <rdfs:comment>A type of red grape used to make a particular red wine.</rdfs:comment>
    </owl:Class>
    


    <!-- http://www.semanticweb.org/danielperez-milasanchez/ontologies/2023/3/untitled-ontology-5#Monastrell_red_grape -->


    <owl:Class rdf:about="http://www.semanticweb.org/danielperez-milasanchez/ontologies/2023/3/untitled-ontology-5#Monastrell_red_grape">
        <rdfs:subClassOf rdf:resource="http://www.semanticweb.org/danielperez-milasanchez/ontologies/2023/3/untitled-ontology-5#Red_grape"/>
        <rdfs:comment>A type of red grape used to make a particular red wine.</rdfs:comment>
    </owl:Class>
    


    <!-- http://www.semanticweb.org/danielperez-milasanchez/ontologies/2023/3/untitled-ontology-5#Monastrell_wine -->


    <owl:Class rdf:about="http://www.semanticweb.org/danielperez-milasanchez/ontologies/2023/3/untitled-ontology-5#Monastrell_wine">
        <rdfs:subClassOf rdf:resource="http://www.semanticweb.org/danielperez-milasanchez/ontologies/2023/3/untitled-ontology-5#Red_wine"/>
        <rdfs:comment>A deeply bold, smoky red wine found in abundance in Central Spain and Southern France (where it’s known as Mourvèdre). Monastrell is the “M” in the Rhône / GSM blend.</rdfs:comment>
    </owl:Class>
    


    <!-- http://www.semanticweb.org/danielperez-milasanchez/ontologies/2023/3/untitled-ontology-5#Montsant_Red_wine -->


    <owl:Class rdf:about="http://www.semanticweb.org/danielperez-milasanchez/ontologies/2023/3/untitled-ontology-5#Montsant_Red_wine">
        <rdfs:subClassOf rdf:resource="http://www.semanticweb.org/danielperez-milasanchez/ontologies/2023/3/untitled-ontology-5#Red_wine"/>
        <rdfs:comment>Montsant is a Spanish Denominación de Origen Protegida (DOP) for wine located in the province of Tarragona and covers 12 municipalities.</rdfs:comment>
    </owl:Class>
    


    <!-- http://www.semanticweb.org/danielperez-milasanchez/ontologies/2023/3/untitled-ontology-5#Moscatell_of_Alexandria_white_grape -->


    <owl:Class rdf:about="http://www.semanticweb.org/danielperez-milasanchez/ontologies/2023/3/untitled-ontology-5#Moscatell_of_Alexandria_white_grape">
        <rdfs:subClassOf rdf:resource="http://www.semanticweb.org/danielperez-milasanchez/ontologies/2023/3/untitled-ontology-5#White_grape"/>
        <rdfs:comment>A type of white grape used to make a particular white or sparkling wine.</rdfs:comment>
    </owl:Class>
    


    <!-- http://www.semanticweb.org/danielperez-milasanchez/ontologies/2023/3/untitled-ontology-5#Navarre -->


    <owl:Class rdf:about="http://www.semanticweb.org/danielperez-milasanchez/ontologies/2023/3/untitled-ontology-5#Navarre">
        <rdfs:subClassOf rdf:resource="http://www.semanticweb.org/danielperez-milasanchez/ontologies/2023/3/untitled-ontology-5#Spanish_region"/>
        <rdfs:comment>It is an Autonomous Community of Spain where grapes are grown for wine production.</rdfs:comment>
    </owl:Class>
    


    <!-- http://www.semanticweb.org/danielperez-milasanchez/ontologies/2023/3/untitled-ontology-5#Parellada_white_grape -->


    <owl:Class rdf:about="http://www.semanticweb.org/danielperez-milasanchez/ontologies/2023/3/untitled-ontology-5#Parellada_white_grape">
        <rdfs:subClassOf rdf:resource="http://www.semanticweb.org/danielperez-milasanchez/ontologies/2023/3/untitled-ontology-5#White_grape"/>
        <rdfs:comment>A type of white grape used to make a particular white or sparkling wine.</rdfs:comment>
    </owl:Class>
    


    <!-- http://www.semanticweb.org/danielperez-milasanchez/ontologies/2023/3/untitled-ontology-5#Pedro_Ximenez_grape -->


    <owl:Class rdf:about="http://www.semanticweb.org/danielperez-milasanchez/ontologies/2023/3/untitled-ontology-5#Pedro_Ximenez_grape">
        <rdfs:subClassOf rdf:resource="http://www.semanticweb.org/danielperez-milasanchez/ontologies/2023/3/untitled-ontology-5#White_grape"/>
        <rdfs:comment>A type of white grape used to make a particular white or Sherry wine.</rdfs:comment>
    </owl:Class>
    


    <!-- http://www.semanticweb.org/danielperez-milasanchez/ontologies/2023/3/untitled-ontology-5#Pedro_Ximenez_wine -->


    <owl:Class rdf:about="http://www.semanticweb.org/danielperez-milasanchez/ontologies/2023/3/untitled-ontology-5#Pedro_Ximenez_wine">
        <rdfs:subClassOf rdf:resource="http://www.semanticweb.org/danielperez-milasanchez/ontologies/2023/3/untitled-ontology-5#Sherry_wine"/>
        <rdfs:comment>The Andalucían grapes responsible for some of the world’s sweetest fortified wines are often dried in the sun to further concentrate the sugars.</rdfs:comment>
    </owl:Class>
    


    <!-- http://www.semanticweb.org/danielperez-milasanchez/ontologies/2023/3/untitled-ontology-5#Priorat_Red_wine -->


    <owl:Class rdf:about="http://www.semanticweb.org/danielperez-milasanchez/ontologies/2023/3/untitled-ontology-5#Priorat_Red_wine">
        <rdfs:subClassOf rdf:resource="http://www.semanticweb.org/danielperez-milasanchez/ontologies/2023/3/untitled-ontology-5#Red_wine"/>
        <rdfs:comment>Priorat is a Denominació d&apos;Origen Qualificada (DOQ) for Catalan wines produced in the Priorat county, in the province of Tarragona, in the southwest of Catalonia.</rdfs:comment>
    </owl:Class>
    


    <!-- http://www.semanticweb.org/danielperez-milasanchez/ontologies/2023/3/untitled-ontology-5#Red_grape -->


    <owl:Class rdf:about="http://www.semanticweb.org/danielperez-milasanchez/ontologies/2023/3/untitled-ontology-5#Red_grape">
        <rdfs:subClassOf rdf:resource="http://www.semanticweb.org/danielperez-milasanchez/ontologies/2023/3/untitled-ontology-5#Grape"/>
        <owl:disjointWith rdf:resource="http://www.semanticweb.org/danielperez-milasanchez/ontologies/2023/3/untitled-ontology-5#White_grape"/>
        <rdfs:comment>Grapes are small dark purple fruit which grow in bunches.</rdfs:comment>
    </owl:Class>
    


    <!-- http://www.semanticweb.org/danielperez-milasanchez/ontologies/2023/3/untitled-ontology-5#Red_wine -->


    <owl:Class rdf:about="http://www.semanticweb.org/danielperez-milasanchez/ontologies/2023/3/untitled-ontology-5#Red_wine">
        <rdfs:subClassOf rdf:resource="http://www.semanticweb.org/danielperez-milasanchez/ontologies/2023/3/untitled-ontology-5#Wine"/>
        <rdfs:comment>Wines made with red grapes (Pinot Noir, Cabernet Sauvignon, etc.).</rdfs:comment>
    </owl:Class>
    


    <!-- http://www.semanticweb.org/danielperez-milasanchez/ontologies/2023/3/untitled-ontology-5#Ribera_del_Duero_Red_wine -->


    <owl:Class rdf:about="http://www.semanticweb.org/danielperez-milasanchez/ontologies/2023/3/untitled-ontology-5#Ribera_del_Duero_Red_wine">
        <rdfs:subClassOf rdf:resource="http://www.semanticweb.org/danielperez-milasanchez/ontologies/2023/3/untitled-ontology-5#Red_wine"/>
        <rdfs:comment>Ribera del Duero is a Spanish Denominación de Origen Protegida (DOP) located in the country&apos;s northern plateau and is one of eleven &apos;quality wine&apos; regions within the autonomous community of Castile and León.</rdfs:comment>
    </owl:Class>
    


    <!-- http://www.semanticweb.org/danielperez-milasanchez/ontologies/2023/3/untitled-ontology-5#Rioja_Red_wine -->


    <owl:Class rdf:about="http://www.semanticweb.org/danielperez-milasanchez/ontologies/2023/3/untitled-ontology-5#Rioja_Red_wine">
        <rdfs:subClassOf rdf:resource="http://www.semanticweb.org/danielperez-milasanchez/ontologies/2023/3/untitled-ontology-5#Red_wine"/>
        <rdfs:comment>Rioja is a wine region in Spain, with denominación de origen calificada. Rioja wine is made from grapes grown in the autonomous communities of La Rioja and Navarre, and the Basque province of Álava.</rdfs:comment>
    </owl:Class>
    


    <!-- http://www.semanticweb.org/danielperez-milasanchez/ontologies/2023/3/untitled-ontology-5#Rioja_White_wine -->


    <owl:Class rdf:about="http://www.semanticweb.org/danielperez-milasanchez/ontologies/2023/3/untitled-ontology-5#Rioja_White_wine">
        <rdfs:subClassOf rdf:resource="http://www.semanticweb.org/danielperez-milasanchez/ontologies/2023/3/untitled-ontology-5#White_wine"/>
        <rdfs:comment>Rioja is a wine region in Spain, with denominación de origen calificada. Rioja wine is made from grapes grown in the autonomous communities of La Rioja and Navarre, and the Basque province of Álava.</rdfs:comment>
    </owl:Class>
    


    <!-- http://www.semanticweb.org/danielperez-milasanchez/ontologies/2023/3/untitled-ontology-5#Sauvignon_Blanc_wine -->


    <owl:Class rdf:about="http://www.semanticweb.org/danielperez-milasanchez/ontologies/2023/3/untitled-ontology-5#Sauvignon_Blanc_wine">
        <rdfs:subClassOf rdf:resource="http://www.semanticweb.org/danielperez-milasanchez/ontologies/2023/3/untitled-ontology-5#White_wine"/>
        <rdfs:comment>A popular and unmistakable white wine that’s loved for its “green” herbal flavors and racy acidity. Sauvignon Blanc grows nearly everywhere and thus, offers a variety of styles ranging from lean to bountiful.</rdfs:comment>
    </owl:Class>
    


    <!-- http://www.semanticweb.org/danielperez-milasanchez/ontologies/2023/3/untitled-ontology-5#Sauvignon_white_grape -->


    <owl:Class rdf:about="http://www.semanticweb.org/danielperez-milasanchez/ontologies/2023/3/untitled-ontology-5#Sauvignon_white_grape">
        <rdfs:subClassOf rdf:resource="http://www.semanticweb.org/danielperez-milasanchez/ontologies/2023/3/untitled-ontology-5#White_grape"/>
        <rdfs:comment>A type of white grape used to make a particular white or sparkling wine.</rdfs:comment>
    </owl:Class>
    


    <!-- http://www.semanticweb.org/danielperez-milasanchez/ontologies/2023/3/untitled-ontology-5#Sherry_wine -->


    <owl:Class rdf:about="http://www.semanticweb.org/danielperez-milasanchez/ontologies/2023/3/untitled-ontology-5#Sherry_wine">
        <rdfs:subClassOf rdf:resource="http://www.semanticweb.org/danielperez-milasanchez/ontologies/2023/3/untitled-ontology-5#Wine"/>
        <rdfs:comment>Sherry is a fortified wine made from white grapes that are grown near the city of Jerez de la Frontera in Andalusia, Spain. Sherry is produced in a variety of styles made primarily from the Palomino grape, ranging from light versions similar to white table wines, such as Manzanilla and fino, to darker and heavier versions that have been allowed to oxidise as they age in barrel, such as Amontillado and oloroso.</rdfs:comment>
    </owl:Class>
    


    <!-- http://www.semanticweb.org/danielperez-milasanchez/ontologies/2023/3/untitled-ontology-5#Spanish_region -->


    <owl:Class rdf:about="http://www.semanticweb.org/danielperez-milasanchez/ontologies/2023/3/untitled-ontology-5#Spanish_region">
        <rdfs:comment>Spanish regions are called Autonomous Communities.</rdfs:comment>
    </owl:Class>
    


    <!-- http://www.semanticweb.org/danielperez-milasanchez/ontologies/2023/3/untitled-ontology-5#Sparkling_wine -->


    <owl:Class rdf:about="http://www.semanticweb.org/danielperez-milasanchez/ontologies/2023/3/untitled-ontology-5#Sparkling_wine">
        <rdfs:subClassOf rdf:resource="http://www.semanticweb.org/danielperez-milasanchez/ontologies/2023/3/untitled-ontology-5#Wine"/>
        <rdfs:comment>Wines having bubbles created by natural fermentation. All champagnes are sparkling wines, but not all sparkling wines are champagnes.</rdfs:comment>
    </owl:Class>
    


    <!-- http://www.semanticweb.org/danielperez-milasanchez/ontologies/2023/3/untitled-ontology-5#Syrah_red_grape -->


    <owl:Class rdf:about="http://www.semanticweb.org/danielperez-milasanchez/ontologies/2023/3/untitled-ontology-5#Syrah_red_grape">
        <rdfs:subClassOf rdf:resource="http://www.semanticweb.org/danielperez-milasanchez/ontologies/2023/3/untitled-ontology-5#Red_grape"/>
        <rdfs:comment>A type of red grape used to make a particular red wine.</rdfs:comment>
    </owl:Class>
    


    <!-- http://www.semanticweb.org/danielperez-milasanchez/ontologies/2023/3/untitled-ontology-5#Syrah_wine -->


    <owl:Class rdf:about="http://www.semanticweb.org/danielperez-milasanchez/ontologies/2023/3/untitled-ontology-5#Syrah_wine">
        <rdfs:subClassOf rdf:resource="http://www.semanticweb.org/danielperez-milasanchez/ontologies/2023/3/untitled-ontology-5#Montsant_Red_wine"/>
        <rdfs:subClassOf rdf:resource="http://www.semanticweb.org/danielperez-milasanchez/ontologies/2023/3/untitled-ontology-5#Priorat_Red_wine"/>
        <rdfs:subClassOf rdf:resource="http://www.semanticweb.org/danielperez-milasanchez/ontologies/2023/3/untitled-ontology-5#Red_wine"/>
        <rdfs:comment>A rich, powerful, and sometimes meaty red wine that originated in the Rhône Valley of France. Syrah is the most planted grape of Australia, where they call it Shiraz.</rdfs:comment>
    </owl:Class>
    


    <!-- http://www.semanticweb.org/danielperez-milasanchez/ontologies/2023/3/untitled-ontology-5#Tempranillo_red_grape -->


    <owl:Class rdf:about="http://www.semanticweb.org/danielperez-milasanchez/ontologies/2023/3/untitled-ontology-5#Tempranillo_red_grape">
        <rdfs:subClassOf rdf:resource="http://www.semanticweb.org/danielperez-milasanchez/ontologies/2023/3/untitled-ontology-5#Red_grape"/>
        <rdfs:comment>A type of red grape used to make a particular red wine.</rdfs:comment>
    </owl:Class>
    


    <!-- http://www.semanticweb.org/danielperez-milasanchez/ontologies/2023/3/untitled-ontology-5#Tempranillo_wine -->


    <owl:Class rdf:about="http://www.semanticweb.org/danielperez-milasanchez/ontologies/2023/3/untitled-ontology-5#Tempranillo_wine">
        <rdfs:subClassOf rdf:resource="http://www.semanticweb.org/danielperez-milasanchez/ontologies/2023/3/untitled-ontology-5#Montsant_Red_wine"/>
        <rdfs:subClassOf rdf:resource="http://www.semanticweb.org/danielperez-milasanchez/ontologies/2023/3/untitled-ontology-5#Red_wine"/>
        <rdfs:subClassOf rdf:resource="http://www.semanticweb.org/danielperez-milasanchez/ontologies/2023/3/untitled-ontology-5#Ribera_del_Duero_Red_wine"/>
        <rdfs:subClassOf rdf:resource="http://www.semanticweb.org/danielperez-milasanchez/ontologies/2023/3/untitled-ontology-5#Rioja_Red_wine"/>
        <rdfs:comment>Spain’s top red wine, made famous by Rioja, where wines are classified (in part) by how long they age in oak. What’s amazing, is a well-made Tempranillo ages for over 20 years.</rdfs:comment>
    </owl:Class>
    


    <!-- http://www.semanticweb.org/danielperez-milasanchez/ontologies/2023/3/untitled-ontology-5#Toro_Red_wine -->


    <owl:Class rdf:about="http://www.semanticweb.org/danielperez-milasanchez/ontologies/2023/3/untitled-ontology-5#Toro_Red_wine">
        <rdfs:subClassOf rdf:resource="http://www.semanticweb.org/danielperez-milasanchez/ontologies/2023/3/untitled-ontology-5#Red_wine"/>
        <rdfs:comment>Toro is a Spanish Denominación de Origen Protegida (DOP) for wines in the province of Zamora, which is in the northwest of Castile and Léon (Spain). The area covered by the DOP is in the southeastern corner of Zamora province and includes the lands known as Tierra del Vino, Valle del Guareña and Tierra de Toro.</rdfs:comment>
    </owl:Class>
    


    <!-- http://www.semanticweb.org/danielperez-milasanchez/ontologies/2023/3/untitled-ontology-5#Toro_red_grape -->


    <owl:Class rdf:about="http://www.semanticweb.org/danielperez-milasanchez/ontologies/2023/3/untitled-ontology-5#Toro_red_grape">
        <rdfs:subClassOf rdf:resource="http://www.semanticweb.org/danielperez-milasanchez/ontologies/2023/3/untitled-ontology-5#Red_grape"/>
        <rdfs:comment>A type of red grape used to make a particular red wine.</rdfs:comment>
    </owl:Class>
    


    <!-- http://www.semanticweb.org/danielperez-milasanchez/ontologies/2023/3/untitled-ontology-5#Valencia -->


    <owl:Class rdf:about="http://www.semanticweb.org/danielperez-milasanchez/ontologies/2023/3/untitled-ontology-5#Valencia">
        <rdfs:subClassOf rdf:resource="http://www.semanticweb.org/danielperez-milasanchez/ontologies/2023/3/untitled-ontology-5#Spanish_region"/>
        <rdfs:comment>It is an Autonomous Community of Spain where grapes are grown for wine production.</rdfs:comment>
    </owl:Class>
    


    <!-- http://www.semanticweb.org/danielperez-milasanchez/ontologies/2023/3/untitled-ontology-5#Verdejo_white_grape -->


    <owl:Class rdf:about="http://www.semanticweb.org/danielperez-milasanchez/ontologies/2023/3/untitled-ontology-5#Verdejo_white_grape">
        <rdfs:subClassOf rdf:resource="http://www.semanticweb.org/danielperez-milasanchez/ontologies/2023/3/untitled-ontology-5#White_grape"/>
        <rdfs:comment>A type of white grape used to make a particular white or sparkling wine.</rdfs:comment>
    </owl:Class>
    


    <!-- http://www.semanticweb.org/danielperez-milasanchez/ontologies/2023/3/untitled-ontology-5#Verdejo_wine -->


    <owl:Class rdf:about="http://www.semanticweb.org/danielperez-milasanchez/ontologies/2023/3/untitled-ontology-5#Verdejo_wine">
        <rdfs:subClassOf rdf:resource="http://www.semanticweb.org/danielperez-milasanchez/ontologies/2023/3/untitled-ontology-5#White_wine"/>
        <rdfs:comment>An herbaceous white wine that grows almost exclusively in the Rueda region of Spain. Not to be confused with Verdelho, a Portuguese grape used in primarily in Madeira.</rdfs:comment>
    </owl:Class>
    


    <!-- http://www.semanticweb.org/danielperez-milasanchez/ontologies/2023/3/untitled-ontology-5#Viura_white_grape -->


    <owl:Class rdf:about="http://www.semanticweb.org/danielperez-milasanchez/ontologies/2023/3/untitled-ontology-5#Viura_white_grape">
        <rdfs:subClassOf rdf:resource="http://www.semanticweb.org/danielperez-milasanchez/ontologies/2023/3/untitled-ontology-5#White_grape"/>
        <rdfs:comment>A type of white grape used to make a particular white or sparkling wine.</rdfs:comment>
    </owl:Class>
    


    <!-- http://www.semanticweb.org/danielperez-milasanchez/ontologies/2023/3/untitled-ontology-5#White_grape -->


    <owl:Class rdf:about="http://www.semanticweb.org/danielperez-milasanchez/ontologies/2023/3/untitled-ontology-5#White_grape">
        <rdfs:subClassOf rdf:resource="http://www.semanticweb.org/danielperez-milasanchez/ontologies/2023/3/untitled-ontology-5#Grape"/>
        <rdfs:comment>Grapes are small green fruit which grow in bunches.</rdfs:comment>
    </owl:Class>
    


    <!-- http://www.semanticweb.org/danielperez-milasanchez/ontologies/2023/3/untitled-ontology-5#White_wine -->


    <owl:Class rdf:about="http://www.semanticweb.org/danielperez-milasanchez/ontologies/2023/3/untitled-ontology-5#White_wine">
        <rdfs:subClassOf rdf:resource="http://www.semanticweb.org/danielperez-milasanchez/ontologies/2023/3/untitled-ontology-5#Wine"/>
        <rdfs:comment>Wines made with white grapes (Albariño, Chardonnay, etc.).</rdfs:comment>
    </owl:Class>
    


    <!-- http://www.semanticweb.org/danielperez-milasanchez/ontologies/2023/3/untitled-ontology-5#Wine -->


    <owl:Class rdf:about="http://www.semanticweb.org/danielperez-milasanchez/ontologies/2023/3/untitled-ontology-5#Wine">
        <owl:equivalentClass>
            <owl:Restriction>
                <owl:onProperty rdf:resource="http://www.semanticweb.org/danielperez-milasanchez/ontologies/2023/3/untitled-ontology-5#isComposedOf"/>
                <owl:someValuesFrom rdf:resource="http://www.semanticweb.org/danielperez-milasanchez/ontologies/2023/3/untitled-ontology-5#Grape"/>
            </owl:Restriction>
        </owl:equivalentClass>
        <owl:equivalentClass>
            <owl:Restriction>
                <owl:onProperty rdf:resource="http://www.semanticweb.org/danielperez-milasanchez/ontologies/2023/3/untitled-ontology-5#isMadeIn"/>
                <owl:someValuesFrom rdf:resource="http://www.semanticweb.org/danielperez-milasanchez/ontologies/2023/3/untitled-ontology-5#Spanish_region"/>
            </owl:Restriction>
        </owl:equivalentClass>
        <owl:equivalentClass>
            <owl:Restriction>
                <owl:onProperty rdf:resource="http://www.semanticweb.org/danielperez-milasanchez/ontologies/2023/3/untitled-ontology-5#hasAcidityLevel"/>
                <owl:someValuesFrom>
                    <rdfs:Datatype>
                        <owl:onDatatype rdf:resource="http://www.w3.org/2001/XMLSchema#int"/>
                        <owl:withRestrictions rdf:parseType="Collection">
                            <rdf:Description>
                                <xsd:minInclusive rdf:datatype="http://www.w3.org/2001/XMLSchema#int">1</xsd:minInclusive>
                            </rdf:Description>
                            <rdf:Description>
                                <xsd:maxInclusive rdf:datatype="http://www.w3.org/2001/XMLSchema#int">5</xsd:maxInclusive>
                            </rdf:Description>
                        </owl:withRestrictions>
                    </rdfs:Datatype>
                </owl:someValuesFrom>
            </owl:Restriction>
        </owl:equivalentClass>
        <owl:equivalentClass>
            <owl:Restriction>
                <owl:onProperty rdf:resource="http://www.semanticweb.org/danielperez-milasanchez/ontologies/2023/3/untitled-ontology-5#hasAlcoholDegree"/>
                <owl:someValuesFrom>
                    <rdfs:Datatype>
                        <owl:onDatatype rdf:resource="http://www.w3.org/2001/XMLSchema#float"/>
                        <owl:withRestrictions rdf:parseType="Collection">
                            <rdf:Description>
                                <xsd:minInclusive rdf:datatype="http://www.w3.org/2001/XMLSchema#float">0.0</xsd:minInclusive>
                            </rdf:Description>
                            <rdf:Description>
                                <xsd:maxInclusive rdf:datatype="http://www.w3.org/2001/XMLSchema#float">100.0</xsd:maxInclusive>
                            </rdf:Description>
                        </owl:withRestrictions>
                    </rdfs:Datatype>
                </owl:someValuesFrom>
            </owl:Restriction>
        </owl:equivalentClass>
        <owl:equivalentClass>
            <owl:Restriction>
                <owl:onProperty rdf:resource="http://www.semanticweb.org/danielperez-milasanchez/ontologies/2023/3/untitled-ontology-5#hasBodyLevel"/>
                <owl:someValuesFrom>
                    <rdfs:Datatype>
                        <owl:onDatatype rdf:resource="http://www.w3.org/2001/XMLSchema#int"/>
                        <owl:withRestrictions rdf:parseType="Collection">
                            <rdf:Description>
                                <xsd:minInclusive rdf:datatype="http://www.w3.org/2001/XMLSchema#int">1</xsd:minInclusive>
                            </rdf:Description>
                            <rdf:Description>
                                <xsd:maxInclusive rdf:datatype="http://www.w3.org/2001/XMLSchema#int">5</xsd:maxInclusive>
                            </rdf:Description>
                        </owl:withRestrictions>
                    </rdfs:Datatype>
                </owl:someValuesFrom>
            </owl:Restriction>
        </owl:equivalentClass>
        <owl:equivalentClass>
            <owl:Restriction>
                <owl:onProperty rdf:resource="http://www.semanticweb.org/danielperez-milasanchez/ontologies/2023/3/untitled-ontology-5#hasAcidityLevel"/>
                <owl:qualifiedCardinality rdf:datatype="http://www.w3.org/2001/XMLSchema#nonNegativeInteger">1</owl:qualifiedCardinality>
                <owl:onDataRange rdf:resource="http://www.w3.org/2001/XMLSchema#int"/>
            </owl:Restriction>
        </owl:equivalentClass>
        <owl:equivalentClass>
            <owl:Restriction>
                <owl:onProperty rdf:resource="http://www.semanticweb.org/danielperez-milasanchez/ontologies/2023/3/untitled-ontology-5#hasAlcoholDegree"/>
                <owl:qualifiedCardinality rdf:datatype="http://www.w3.org/2001/XMLSchema#nonNegativeInteger">1</owl:qualifiedCardinality>
                <owl:onDataRange rdf:resource="http://www.w3.org/2001/XMLSchema#float"/>
            </owl:Restriction>
        </owl:equivalentClass>
        <owl:equivalentClass>
            <owl:Restriction>
                <owl:onProperty rdf:resource="http://www.semanticweb.org/danielperez-milasanchez/ontologies/2023/3/untitled-ontology-5#hasBodyLevel"/>
                <owl:qualifiedCardinality rdf:datatype="http://www.w3.org/2001/XMLSchema#nonNegativeInteger">1</owl:qualifiedCardinality>
                <owl:onDataRange rdf:resource="http://www.w3.org/2001/XMLSchema#int"/>
            </owl:Restriction>
        </owl:equivalentClass>
        <rdfs:comment>Wine is an alcoholic drink typically made from fermented grapes. Yeast consumes the sugar in the grapes and converts it to ethanol and carbon dioxide, releasing heat in the process.</rdfs:comment>
    </owl:Class>
    


    <!-- 
    ///////////////////////////////////////////////////////////////////////////////////////
    //
    // Individuals
    //
    ///////////////////////////////////////////////////////////////////////////////////////
     -->


    


    <!-- http://www.semanticweb.org/danielperez-milasanchez/ontologies/2023/3/untitled-ontology-5#Andalusia -->


    <owl:NamedIndividual rdf:about="http://www.semanticweb.org/danielperez-milasanchez/ontologies/2023/3/untitled-ontology-5#Andalusia">
        <rdf:type rdf:resource="http://www.semanticweb.org/danielperez-milasanchez/ontologies/2023/3/untitled-ontology-5#Andalusia"/>
    </owl:NamedIndividual>
    


    <!-- http://www.semanticweb.org/danielperez-milasanchez/ontologies/2023/3/untitled-ontology-5#CandL -->


    <owl:NamedIndividual rdf:about="http://www.semanticweb.org/danielperez-milasanchez/ontologies/2023/3/untitled-ontology-5#CandL">
        <rdf:type rdf:resource="http://www.semanticweb.org/danielperez-milasanchez/ontologies/2023/3/untitled-ontology-5#Castile_and_Leon"/>
    </owl:NamedIndividual>
    


    <!-- http://www.semanticweb.org/danielperez-milasanchez/ontologies/2023/3/untitled-ontology-5#Test -->


    <owl:NamedIndividual rdf:about="http://www.semanticweb.org/danielperez-milasanchez/ontologies/2023/3/untitled-ontology-5#Test">
        <isComposedOf rdf:resource="http://www.semanticweb.org/danielperez-milasanchez/ontologies/2023/3/untitled-ontology-5#grape_test"/>
        <isComposedOf rdf:resource="http://www.semanticweb.org/danielperez-milasanchez/ontologies/2023/3/untitled-ontology-5#grape_test_2"/>
        <hasAcidityLevel rdf:datatype="http://www.w3.org/2001/XMLSchema#int">5</hasAcidityLevel>
        <hasAlcoholDegree rdf:datatype="http://www.w3.org/2001/XMLSchema#float">60.0</hasAlcoholDegree>
    </owl:NamedIndividual>
    


    <!-- http://www.semanticweb.org/danielperez-milasanchez/ontologies/2023/3/untitled-ontology-5#grape_test -->


    <owl:NamedIndividual rdf:about="http://www.semanticweb.org/danielperez-milasanchez/ontologies/2023/3/untitled-ontology-5#grape_test">
        <isGrownIn rdf:resource="http://www.semanticweb.org/danielperez-milasanchez/ontologies/2023/3/untitled-ontology-5#Andalusia"/>
    </owl:NamedIndividual>
    


    <!-- http://www.semanticweb.org/danielperez-milasanchez/ontologies/2023/3/untitled-ontology-5#grape_test_2 -->


    <owl:NamedIndividual rdf:about="http://www.semanticweb.org/danielperez-milasanchez/ontologies/2023/3/untitled-ontology-5#grape_test_2">
        <rdf:type rdf:resource="http://www.semanticweb.org/danielperez-milasanchez/ontologies/2023/3/untitled-ontology-5#Red_grape"/>
        <isGrownIn rdf:resource="http://www.semanticweb.org/danielperez-milasanchez/ontologies/2023/3/untitled-ontology-5#CandL"/>
    </owl:NamedIndividual>
    


    <!-- 
    ///////////////////////////////////////////////////////////////////////////////////////
    //
    // Annotations
    //
    ///////////////////////////////////////////////////////////////////////////////////////
     -->


    <rdf:Description rdf:about="http://www.semanticweb.org/danielperez-milasanchez/ontologies/2023/3/untitled-ontology-5#Andalusia">
        <rdfs:comment>It is an Autonomous Community of Spain where grapes are grown for wine production.</rdfs:comment>
    </rdf:Description>
    <rdf:Description rdf:about="http://www.w3.org/2002/07/owl#Thing">
        <rdfs:comment>Main Superclass.</rdfs:comment>
    </rdf:Description>
    


    <!-- 
    ///////////////////////////////////////////////////////////////////////////////////////
    //
    // General axioms
    //
    ///////////////////////////////////////////////////////////////////////////////////////
     -->


    <rdf:Description>
        <rdf:type rdf:resource="http://www.w3.org/2002/07/owl#AllDisjointClasses"/>
        <owl:members rdf:parseType="Collection">
            <rdf:Description rdf:about="http://www.semanticweb.org/danielperez-milasanchez/ontologies/2023/3/untitled-ontology-5#Grape"/>
            <rdf:Description rdf:about="http://www.semanticweb.org/danielperez-milasanchez/ontologies/2023/3/untitled-ontology-5#Spanish_region"/>
            <rdf:Description rdf:about="http://www.semanticweb.org/danielperez-milasanchez/ontologies/2023/3/untitled-ontology-5#Wine"/>
        </owl:members>
    </rdf:Description>
    <rdf:Description>
        <rdf:type rdf:resource="http://www.w3.org/2002/07/owl#AllDisjointClasses"/>
        <owl:members rdf:parseType="Collection">
            <rdf:Description rdf:about="http://www.semanticweb.org/danielperez-milasanchez/ontologies/2023/3/untitled-ontology-5#Red_wine"/>
            <rdf:Description rdf:about="http://www.semanticweb.org/danielperez-milasanchez/ontologies/2023/3/untitled-ontology-5#Sherry_wine"/>
            <rdf:Description rdf:about="http://www.semanticweb.org/danielperez-milasanchez/ontologies/2023/3/untitled-ontology-5#Sparkling_wine"/>
            <rdf:Description rdf:about="http://www.semanticweb.org/danielperez-milasanchez/ontologies/2023/3/untitled-ontology-5#White_wine"/>
        </owl:members>
    </rdf:Description>
    


    <!-- 
    ///////////////////////////////////////////////////////////////////////////////////////
    //
    // Rules
    //
    ///////////////////////////////////////////////////////////////////////////////////////
     -->


    <rdf:Description rdf:about="urn:swrl:var#w">
        <rdf:type rdf:resource="http://www.w3.org/2003/11/swrl#Variable"/>
    </rdf:Description>
    <rdf:Description rdf:about="urn:swrl:var#g">
        <rdf:type rdf:resource="http://www.w3.org/2003/11/swrl#Variable"/>
    </rdf:Description>
    <rdf:Description rdf:about="urn:swrl:var#r">
        <rdf:type rdf:resource="http://www.w3.org/2003/11/swrl#Variable"/>
    </rdf:Description>
    <rdf:Description>
        <rdf:type rdf:resource="http://www.w3.org/2003/11/swrl#Imp"/>
        <swrl:body>
            <rdf:Description>
                <rdf:type rdf:resource="http://www.w3.org/2003/11/swrl#AtomList"/>
                <rdf:first>
                    <rdf:Description>
                        <rdf:type rdf:resource="http://www.w3.org/2003/11/swrl#ClassAtom"/>
                        <swrl:classPredicate rdf:resource="http://www.semanticweb.org/danielperez-milasanchez/ontologies/2023/3/untitled-ontology-5#Red_wine"/>
                        <swrl:argument1 rdf:resource="urn:swrl:var#w"/>
                    </rdf:Description>
                </rdf:first>
                <rdf:rest>
                    <rdf:Description>
                        <rdf:type rdf:resource="http://www.w3.org/2003/11/swrl#AtomList"/>
                        <rdf:first>
                            <rdf:Description>
                                <rdf:type rdf:resource="http://www.w3.org/2003/11/swrl#IndividualPropertyAtom"/>
                                <swrl:propertyPredicate rdf:resource="http://www.semanticweb.org/danielperez-milasanchez/ontologies/2023/3/untitled-ontology-5#isComposedOf"/>
                                <swrl:argument1 rdf:resource="urn:swrl:var#w"/>
                                <swrl:argument2 rdf:resource="urn:swrl:var#g"/>
                            </rdf:Description>
                        </rdf:first>
                        <rdf:rest>
                            <rdf:Description>
                                <rdf:type rdf:resource="http://www.w3.org/2003/11/swrl#AtomList"/>
                                <rdf:first>
                                    <rdf:Description>
                                        <rdf:type rdf:resource="http://www.w3.org/2003/11/swrl#ClassAtom"/>
                                        <swrl:classPredicate rdf:resource="http://www.semanticweb.org/danielperez-milasanchez/ontologies/2023/3/untitled-ontology-5#Grape"/>
                                        <swrl:argument1 rdf:resource="urn:swrl:var#g"/>
                                    </rdf:Description>
                                </rdf:first>
                                <rdf:rest rdf:resource="http://www.w3.org/1999/02/22-rdf-syntax-ns#nil"/>
                            </rdf:Description>
                        </rdf:rest>
                    </rdf:Description>
                </rdf:rest>
            </rdf:Description>
        </swrl:body>
        <swrl:head>
            <rdf:Description>
                <rdf:type rdf:resource="http://www.w3.org/2003/11/swrl#AtomList"/>
                <rdf:first>
                    <rdf:Description>
                        <rdf:type rdf:resource="http://www.w3.org/2003/11/swrl#ClassAtom"/>
                        <swrl:classPredicate rdf:resource="http://www.semanticweb.org/danielperez-milasanchez/ontologies/2023/3/untitled-ontology-5#Red_grape"/>
                        <swrl:argument1 rdf:resource="urn:swrl:var#g"/>
                    </rdf:Description>
                </rdf:first>
                <rdf:rest rdf:resource="http://www.w3.org/1999/02/22-rdf-syntax-ns#nil"/>
            </rdf:Description>
        </swrl:head>
    </rdf:Description>
    <rdf:Description>
        <rdf:type rdf:resource="http://www.w3.org/2003/11/swrl#Imp"/>
        <swrl:body>
            <rdf:Description>
                <rdf:type rdf:resource="http://www.w3.org/2003/11/swrl#AtomList"/>
                <rdf:first>
                    <rdf:Description>
                        <rdf:type rdf:resource="http://www.w3.org/2003/11/swrl#ClassAtom"/>
                        <swrl:classPredicate rdf:resource="http://www.semanticweb.org/danielperez-milasanchez/ontologies/2023/3/untitled-ontology-5#White_wine"/>
                        <swrl:argument1 rdf:resource="urn:swrl:var#w"/>
                    </rdf:Description>
                </rdf:first>
                <rdf:rest>
                    <rdf:Description>
                        <rdf:type rdf:resource="http://www.w3.org/2003/11/swrl#AtomList"/>
                        <rdf:first>
                            <rdf:Description>
                                <rdf:type rdf:resource="http://www.w3.org/2003/11/swrl#IndividualPropertyAtom"/>
                                <swrl:propertyPredicate rdf:resource="http://www.semanticweb.org/danielperez-milasanchez/ontologies/2023/3/untitled-ontology-5#isComposedOf"/>
                                <swrl:argument1 rdf:resource="urn:swrl:var#w"/>
                                <swrl:argument2 rdf:resource="urn:swrl:var#g"/>
                            </rdf:Description>
                        </rdf:first>
                        <rdf:rest>
                            <rdf:Description>
                                <rdf:type rdf:resource="http://www.w3.org/2003/11/swrl#AtomList"/>
                                <rdf:first>
                                    <rdf:Description>
                                        <rdf:type rdf:resource="http://www.w3.org/2003/11/swrl#ClassAtom"/>
                                        <swrl:classPredicate rdf:resource="http://www.semanticweb.org/danielperez-milasanchez/ontologies/2023/3/untitled-ontology-5#Grape"/>
                                        <swrl:argument1 rdf:resource="urn:swrl:var#g"/>
                                    </rdf:Description>
                                </rdf:first>
                                <rdf:rest rdf:resource="http://www.w3.org/1999/02/22-rdf-syntax-ns#nil"/>
                            </rdf:Description>
                        </rdf:rest>
                    </rdf:Description>
                </rdf:rest>
            </rdf:Description>
        </swrl:body>
        <swrl:head>
            <rdf:Description>
                <rdf:type rdf:resource="http://www.w3.org/2003/11/swrl#AtomList"/>
                <rdf:first>
                    <rdf:Description>
                        <rdf:type rdf:resource="http://www.w3.org/2003/11/swrl#ClassAtom"/>
                        <swrl:classPredicate rdf:resource="http://www.semanticweb.org/danielperez-milasanchez/ontologies/2023/3/untitled-ontology-5#White_grape"/>
                        <swrl:argument1 rdf:resource="urn:swrl:var#g"/>
                    </rdf:Description>
                </rdf:first>
                <rdf:rest rdf:resource="http://www.w3.org/1999/02/22-rdf-syntax-ns#nil"/>
            </rdf:Description>
        </swrl:head>
    </rdf:Description>
    <rdf:Description>
        <rdf:type rdf:resource="http://www.w3.org/2003/11/swrl#Imp"/>
        <swrl:body>
            <rdf:Description>
                <rdf:type rdf:resource="http://www.w3.org/2003/11/swrl#AtomList"/>
                <rdf:first>
                    <rdf:Description>
                        <rdf:type rdf:resource="http://www.w3.org/2003/11/swrl#ClassAtom"/>
                        <swrl:classPredicate rdf:resource="http://www.semanticweb.org/danielperez-milasanchez/ontologies/2023/3/untitled-ontology-5#Wine"/>
                        <swrl:argument1 rdf:resource="urn:swrl:var#w"/>
                    </rdf:Description>
                </rdf:first>
                <rdf:rest>
                    <rdf:Description>
                        <rdf:type rdf:resource="http://www.w3.org/2003/11/swrl#AtomList"/>
                        <rdf:first>
                            <rdf:Description>
                                <rdf:type rdf:resource="http://www.w3.org/2003/11/swrl#ClassAtom"/>
                                <swrl:classPredicate rdf:resource="http://www.semanticweb.org/danielperez-milasanchez/ontologies/2023/3/untitled-ontology-5#Grape"/>
                                <swrl:argument1 rdf:resource="urn:swrl:var#g"/>
                            </rdf:Description>
                        </rdf:first>
                        <rdf:rest>
                            <rdf:Description>
                                <rdf:type rdf:resource="http://www.w3.org/2003/11/swrl#AtomList"/>
                                <rdf:first>
                                    <rdf:Description>
                                        <rdf:type rdf:resource="http://www.w3.org/2003/11/swrl#IndividualPropertyAtom"/>
                                        <swrl:propertyPredicate rdf:resource="http://www.semanticweb.org/danielperez-milasanchez/ontologies/2023/3/untitled-ontology-5#isGrownIn"/>
                                        <swrl:argument1 rdf:resource="urn:swrl:var#g"/>
                                        <swrl:argument2 rdf:resource="urn:swrl:var#r"/>
                                    </rdf:Description>
                                </rdf:first>
                                <rdf:rest>
                                    <rdf:Description>
                                        <rdf:type rdf:resource="http://www.w3.org/2003/11/swrl#AtomList"/>
                                        <rdf:first>
                                            <rdf:Description>
                                                <rdf:type rdf:resource="http://www.w3.org/2003/11/swrl#ClassAtom"/>
                                                <swrl:classPredicate rdf:resource="http://www.semanticweb.org/danielperez-milasanchez/ontologies/2023/3/untitled-ontology-5#Spanish_region"/>
                                                <swrl:argument1 rdf:resource="urn:swrl:var#r"/>
                                            </rdf:Description>
                                        </rdf:first>
                                        <rdf:rest rdf:resource="http://www.w3.org/1999/02/22-rdf-syntax-ns#nil"/>
                                    </rdf:Description>
                                </rdf:rest>
                            </rdf:Description>
                        </rdf:rest>
                    </rdf:Description>
                </rdf:rest>
            </rdf:Description>
        </swrl:body>
        <swrl:head>
            <rdf:Description>
                <rdf:type rdf:resource="http://www.w3.org/2003/11/swrl#AtomList"/>
                <rdf:first>
                    <rdf:Description>
                        <rdf:type rdf:resource="http://www.w3.org/2003/11/swrl#IndividualPropertyAtom"/>
                        <swrl:propertyPredicate rdf:resource="http://www.semanticweb.org/danielperez-milasanchez/ontologies/2023/3/untitled-ontology-5#isMadeIn"/>
                        <swrl:argument1 rdf:resource="urn:swrl:var#w"/>
                        <swrl:argument2 rdf:resource="urn:swrl:var#r"/>
                    </rdf:Description>
                </rdf:first>
                <rdf:rest rdf:resource="http://www.w3.org/1999/02/22-rdf-syntax-ns#nil"/>
            </rdf:Description>
        </swrl:head>
    </rdf:Description>
</rdf:RDF>



<!-- Generated by the OWL API (version 5.1.18) https://github.com/owlcs/owlapi/ -->


